Make Archi.ptr64 always computable, and reorganize files accordingly: ia32 -> x86/x86_32/x86_64
Having Archi.ptr64 as an opaque Parameter that is determined at run-time depending on compcert.ini is problematic for applications such as VST where functions such as Ctypes.sizeof must compute within Coq.

This commit introduces two versions of the Archi.v file, one for x86 32 bits (with ptr64 := false), one for x86 64 bits (with ptr64 := true).  Unlike previous approaches, no other file is duplicated between these two variants of x86.

While we are at it, I renamed "ia32" into "x86" everywhere.  "ia32" is Intel speak for the 32-bit architecture.  It is not a good name to describe both the 32 and 64 bit architectures.

Finally, .depend is no longer under version control and is regenerated when the target architecture changes.  That's because the location of Archi.v differs between the ports that have 32/64 bit variants (x86 so far) and the ports that have only one bitsize (ARM and PowerPC so far).

driver/Driver.ml
@@ -536,7 +536,7 @@ let _ =
       | "arm"     -> if Configuration.is_big_endian
                      then Machine.arm_bigendian
                      else Machine.arm_littleendian
-      | "ia32"    -> if Configuration.model = "64" then
+      | "x86"     -> if Configuration.model = "64" then
                        Machine.x86_64
                      else
                        if Configuration.abi = "macosx"
